WIP

PDDL_temporal_plan_instantiation.thy
@@ -4,7 +4,25 @@ theory PDDL_temporal_plan_instantiation
     Containers.Containers
 begin
 
-derive (linorder) compare rat
+text \<open>This is the type of propositions, we will use to instantiate the locale\<close>
+type_synonym pr = "object atom formula"
+
+type_synonym suff_cond = "pr list"
+
+text \<open>Note, that this is not the type we will use as @{typ \<open>'snap_action\<close>}}, because we would
+have to implement \<open>at_start\<close> as @{term \<open>fst\<close>}, which would cause it violate injectivity.\<close>
+type_synonym snap = "suff_cond \<times> object ast_effect"
+
+type_synonym dc = "duration_op \<times> rat"
+
+text \<open>This is the actual type of action\<close>
+type_synonym action = "(string \<times> snap \<times> snap \<times> snap \<times> dc option)"
+
+text \<open>This is the actual type we will use to instantiate the locale.\<close>
+type_synonym snap_action = "temporal_annotation \<times> action"
+
+
+derive (linorder) compare rat 
 
 derive (eq) ceq predicate func atom object formula 
 derive ccompare predicate func atom object formula
@@ -13,12 +31,19 @@ derive (rbt) set_impl func atom object formula
 
 derive (rbt) mapping_impl object
 
-derive linorder predicate func object atom "object atom formula"
+derive linorder predicate func object atom "object atom formula" prod list ast_effect duration_op
+
+instantiation rat :: time
+begin
+instance apply standard
+  using dense_order_class.dense apply auto[1]
+  using zero_neq_one[symmetric] by blast
+end
 
 context wf_ast_problem
 begin
 subsection \<open>Propositions\<close>
-definition "objs \<equiv>  set (map fst (consts D @ objects P))"
+definition "objs \<equiv> set (map fst (consts D @ objects P))"
 
 definition "tos = {(ty, obj). obj \<in> objs \<and> is_obj_of_type obj ty}"
 
@@ -30,43 +55,53 @@ definition "eqs \<equiv> {(eqAtm a a)| a. a \<in> objs}"
 
 definition "neqs \<equiv> {(eqAtm a b)| a b. a \<in> objs \<and> b \<in> objs \<and> a \<noteq> b}"
 
-type_synonym pr = "object atom formula"
-
 definition propositions::"pr set" where
 "propositions \<equiv> (\<lambda>x. Not (Atom x)) ` preds \<union> Atom ` preds \<union> (\<lambda>x. Not (Atom x)) ` neqs \<union> Atom ` eqs"
 
 subsection \<open>Actions\<close>
+
+text \<open>If the duration constraint is not instantiable it will invalidate the plan according
+to temporal PDDL semantics. Therefore, we can filter out instantiated actions that have
+such duration constraints.\<close>
+fun dur_const_instantiable::"term duration_constraint \<Rightarrow> (term \<Rightarrow> object) \<Rightarrow> bool" where
+"dur_const_instantiable No_Const _ = True" |
+"dur_const_instantiable (Time_Const op d) _ = True" |
+"dur_const_instantiable (Func_Const op f ps) fun = (
+  case (func_eval (FuncEnt f (map fun ps))) of
+    None \<Rightarrow> False
+  | Some v \<Rightarrow> True
+)"
+
 fun instantiate_duration_constraint::"term duration_constraint \<Rightarrow> (term \<Rightarrow> object) \<Rightarrow> duration_op \<times> (rat option)" where
-"instantiate_duration_constraint No_Const _ = (EQ, Some 0)" |
+"instantiate_duration_constraint No_Const _ = (GEQ, None)" |
 "instantiate_duration_constraint (Time_Const op d) _ = (op, Some d)" |
-"instantiate_duration_constraint (Func_Const op f ps) fun = (
-  (op, func_eval (FuncEnt f (map fun ps)))
-)" 
+"instantiate_duration_constraint (Func_Const op f ps) fun =
+  (op, func_eval (FuncEnt f (map fun ps)))" 
 
 definition "inst_dur_const c f \<equiv> case (instantiate_duration_constraint c f) of
   (op, Some v) \<Rightarrow> Some (op, v)
 | (op, None  ) \<Rightarrow> None"
 
-text \<open>This will not contain any invalid duration constraints. On a theoretical level,
-it is interesting that duration constraints for the propositional actions corresponding to 
-PDDL actions depend on the parameters.\<close>
+text \<open>This will not contain any invalid duration constraints.
+It is interesting that duration constraints for propositional actions corresponding to 
+PDDL actions depend on arguments.\<close>
 definition "pddl_durative_actions \<equiv> {
   (n, inst_snap_action a args At_Start, 
   inst_snap_action a args Over_All, 
-  inst_snap_action a args At_End, v) |
-  a args n params cond eff const tys v substt. 
+  inst_snap_action a args At_End, inst_dur_const const substt) |
+  a args n params cond eff const tys substt. 
     a \<in> set (actions D) 
   \<and> a = Durative_Action_Schema n params const cond eff 
   \<and> tys = map snd params 
   \<and> (tys, args) \<in> ltos 
   \<and> substt = subst_term (the o (map_of (zip (map fst params) args)))
-  \<and> Some v = inst_dur_const const substt }"
+  \<and> dur_const_instantiable const substt}"
 
 definition "none_snap = Ground_Action (Not Bot) (Effect Nil Nil)"
 
 definition "pddl_instant_actions \<equiv>{
   (n, instantiate_action_schema a args, 
-    none_snap, none_snap, (EQ, 0)) |
+    none_snap, none_snap, Some (EQ, 0)) |
   a args n params pre eff tys. 
     a \<in> set (actions D) 
   \<and> a = Simple_Action_Schema n params pre eff 
@@ -100,19 +135,10 @@ fun suff_prop_conds::"'a formula \<Rightarrow> 'a formula set set" where
 "suff_prop_conds (Or a b) = suff_prop_conds a \<union> suff_prop_conds b" |
 "suff_prop_conds (Imp a b) =  negate_sc (suff_prop_conds a) \<union> suff_prop_conds b"
 
-fun snap_actions::"ground_action \<Rightarrow> (object atom formula set \<times> object ast_effect) set" where
-"snap_actions (Ground_Action pre eff) = {(pre', eff)|pre'. pre' \<in> (suff_prop_conds pre)}"
+definition "suff_prop_list f \<equiv> sorted_list_of_set ` (suff_prop_conds f)"
 
-type_synonym suff_cond = "pr set"
-
-text \<open>Note, that this is not the type we will use as @{typ \<open>'snap_action\<close>}}, because we would
-have to implement \<open>at_start\<close> as @{term \<open>fst\<close>}, which would cause it violate injectivity.\<close>
-type_synonym snap = "suff_cond \<times> object ast_effect"
-
-type_synonym dc = "duration_op \<times> rat"
-
-text \<open>This is the actual type of action\<close>
-type_synonym action = "(string \<times> snap \<times> snap \<times> snap \<times> dc)"
+fun snap_actions::"ground_action \<Rightarrow> (object atom formula list \<times> object ast_effect) set" where
+"snap_actions (Ground_Action pre eff) = {(pre', eff)|pre'. pre' \<in> (suff_prop_list pre)}"
 
 definition prop_actions::"action set" where
 "prop_actions = {(n, a', inv', e', c)|n a inv e c a' inv' e'. 
@@ -142,23 +168,24 @@ definition "initial_state \<equiv> initial_state' \<union> {Not goal_lock}"
 text \<open>We now define some actions that will lead to the goal state and will prevent any other snap-actions
 from being executed. This needs some consideration about the manner in which we distinguish these snap-actions.\<close>
 
-definition "goal_conditions \<equiv> suff_prop_conds (goal P)"
+definition "goal_conditions \<equiv> suff_prop_list (goal P)"
 
 abbreviation "goal_eff \<equiv> Effect [goal_lock] [Not goal_lock]"
 
 definition goal_snaps::"snap set" where
 "goal_snaps \<equiv> {(s, goal_eff)|s. s \<in> goal_conditions}"
 
-definition "goal_actions \<equiv> {(''Goal'',gs,gs,gs,(EQ, 0))| gs. gs \<in> goal_snaps}"
+definition "goal_actions \<equiv> {(''Goal'',gs,gs,gs, Some (EQ, 0))| gs. gs \<in> goal_snaps}"
 
 definition "acts \<equiv> prop_actions \<union> goal_actions"
+
+definition "goal_imp \<equiv> {goal_lock}"
 
 text \<open>Lemma: propositional actions and goal actions are disjoint. Proof with auxiliary lemmas: the goal_lock
  is not in the set of PDDL \<open>propositions\<close>. PDDL effects only contain PDDL \<open>propositions\<close>.\<close>
 
 subsection \<open>Snap actions\<close>
 
-type_synonym snap_action = "temporal_annotation \<times> action"
 
 definition "at_start_imp \<equiv> Pair At_Start"
 
@@ -170,7 +197,7 @@ text \<open>Before we can implement \<open>over_all\<close> for @{typ snap_actio
 from @{typ snap} to @{typ pr} for \<open>pre\<close>, \<open>adds\<close>, and \<open>dels\<close> respectively.\<close>
 
 definition snap_pre::"snap \<Rightarrow> pr set" where
-"snap_pre \<equiv> fst"
+"snap_pre \<equiv> set o fst"
 
 fun snap_adds::"snap \<Rightarrow> pr set" where
 "snap_adds (pre, eff) = (set (adds eff)) \<union> (negate_literal ` (set (dels eff)))"
@@ -199,13 +226,12 @@ definition "s_snap \<equiv> fst o snd"
 text \<open>The end snap\<close>
 definition "e_snap \<equiv> fst o snd o snd o snd"
 
-definition over_all::"action \<Rightarrow> pr set" where
-"over_all = snap_pre o o_snap"
+definition over_all_imp::"action \<Rightarrow> pr set" where
+"over_all_imp = snap_pre o o_snap"
 
 fun snap_action_to_snap::"snap_action \<Rightarrow> snap" where
 "snap_action_to_snap (At_Start, act) = s_snap act" |
 "snap_action_to_snap (At_End, act) = e_snap act"
-
 
 text \<open>This is the actual function we will use to instantiate \<open>pre\<close> in the @{term temp_planning_problem} locale.\<close>
 definition snap_action_pre::"snap_action \<Rightarrow> pr set" where
@@ -214,15 +240,317 @@ definition snap_action_pre::"snap_action \<Rightarrow> pr set" where
 definition snap_action_adds::"snap_action \<Rightarrow> pr set" where
 "snap_action_adds \<equiv> snap_adds o snap_action_to_snap"
 
-
 definition snap_action_dels::"snap_action \<Rightarrow> pr set" where
 "snap_action_dels \<equiv> snap_dels o snap_action_to_snap"
 
 subsubsection \<open>Duration bounds\<close>
-text \<open>First, define a function from our notion of a ground action to the \<close>
+text \<open>First, define a function from our notion of a ground action to its duration constraint.\<close>
+
+definition action_consts::"action \<Rightarrow> dc option" where
+"action_consts \<equiv> snd o snd o snd o snd"
+
+text \<open>The duration constraints can be negative. They just can never be satisfied by a valid plan. It
+is also a good idea to set the lower bound to 0.\<close>
+fun dc_to_ul::"dc option \<Rightarrow> rat lower_bound \<times> (rat upper_bound option)" where
+"dc_to_ul (Some (EQ, n)) = (GE n, Some (LE n))" |
+"dc_to_ul (Some (GEQ, n)) = (GE n, None)" |
+"dc_to_ul (Some (LEQ, n)) = (GE 0, Some (LE n))" |
+"dc_to_ul None = (GE 0, None)"
+
+definition "lower_impl \<equiv> fst o dc_to_ul o action_consts"
+definition "upper_impl \<equiv> snd o dc_to_ul o action_consts"
+
+end
+
+context wf_ast_problem
+begin
+
+lemma objs_typed: "obj \<in> objs \<longleftrightarrow> (\<exists>ty. (ty, obj) \<in> tos)" 
+proof (rule iffI)
+  assume a: "obj \<in> objs"
+  hence "obj \<in> set (map fst (consts D @ objects P))" unfolding objs_def by blast
+  with wf_problem[simplified wf_problem_def]
+  obtain t where "map_of (consts D @ objects P) obj = Some t" by fastforce
+  hence "is_obj_of_type obj t" unfolding is_of_type_def objT_alt is_obj_of_type_alt using of_type_refl by simp
+  with a
+  show "\<exists>ty. (ty, obj) \<in> tos" unfolding tos_def by auto
+next
+  assume "\<exists>ty. (ty, obj) \<in> tos"
+  thus "obj \<in> objs" unfolding tos_def by simp
+qed
+
+fun effect_props::"object ast_effect \<Rightarrow> object atom formula set" where
+"effect_props (Effect xs ys) = set xs \<union> set ys"
+
+definition "effect_preds f \<equiv> \<Union> (atoms ` (effect_props f))"
+
+abbreviation "form_preds \<equiv> atoms"
+
+fun ga_preds::"ground_action \<Rightarrow> object atom set" where
+"ga_preds (Ground_Action pre eff) = form_preds pre \<union> effect_preds eff"
+
+lemma typed_args_correct: "(tys, args) \<in> ltos \<longleftrightarrow> list_all2 is_obj_of_type args tys"
+proof (rule iffI) 
+  assume "(tys, args) \<in> ltos"
+  thus "list_all2 is_obj_of_type args tys"
+  unfolding ltos_def tos_def
+    apply (subst list_all2_twist)
+    apply (rule list_all2_mono)
+  by simp+
+next
+  have "obj \<in> objs" if "is_obj_of_type obj ty" for obj ty
+  proof -
+    from that
+    have "is_of_type objT obj ty" using is_obj_of_type_alt by simp
+    then obtain T where
+      "objT obj = Some T"
+      "of_type T ty" unfolding is_of_type_def 
+      by (auto split: option.splits)
+    hence "obj \<in> set (map fst (consts D @ objects P))"
+      unfolding objT_alt using map_of_SomeD by fastforce
+    thus ?thesis unfolding objs_def by blast
+  qed
+  moreover
+  assume "list_all2 is_obj_of_type args tys"
+  ultimately
+  have "list_all2 (\<lambda>obj ty. is_obj_of_type obj ty \<and> obj \<in> objs) args tys" using list_all2_mono by force
+  thus "(tys, args) \<in> ltos" unfolding ltos_def tos_def
+    using list_all2_twist list_all2_mono by fastforce
+qed
 
 
-sublocale temp_planning_problem sorry
+lemma sig_iff: "sig n = Some ts \<longleftrightarrow> PredDecl n ts \<in> set (predicates D)"
+proof (rule iffI)
+  assume "sig n = Some ts"
+  thus "PredDecl n ts \<in> set (predicates D)"
+    unfolding sig_def 
+    apply -
+    apply (drule map_of_SomeD)
+    by (auto split: predicate_decl.splits) 
+next
+  assume "PredDecl n ts \<in> set (predicates D)"
+  hence "(n, ts) \<in> set (map (\<lambda>(PredDecl n ts) \<Rightarrow> (n, ts)) (predicates D))" by force
+  moreover
+  have "distinct (map fst (map (\<lambda>(PredDecl n ts) \<Rightarrow> (n, ts)) (predicates D)))" 
+  proof (subst distinct_map; rule conjI)
+    have distinct_preds: "distinct (predicates D)" using wf_domain unfolding wf_domain_def using distinct_mapI by blast
+    
+    show "distinct (map (case_predicate_decl Pair) (predicates D))" 
+    proof (subst distinct_map; rule conjI)
+      show "distinct (predicates D)" using distinct_preds .
+      have inj_pd: "inj (\<lambda>x. case x of PredDecl n ts \<Rightarrow> (n, ts))" 
+      unfolding inj_def 
+      apply (intro allI) 
+      subgoal for x y
+        by (cases x; cases y) auto
+      done
+    thus "inj_on (case_predicate_decl Pair) (set (predicates D))" unfolding inj_on_def inj_def by simp
+    qed
+    show "inj_on fst (set (map (case_predicate_decl Pair) (predicates D)))" 
+    proof (rule inj_onI)
+      fix x y
+      assume x: "x \<in> set (map (case_predicate_decl Pair) (predicates D))"
+        and  y: "y \<in> set (map (case_predicate_decl Pair) (predicates D))" 
+        and xy: "fst x = fst y"
+      from x
+      obtain px nx vx  where
+        px: "case_predicate_decl Pair px = x"
+        "px \<in> set (predicates D)"
+        "px = PredDecl nx vx"
+        "x = (nx, vx)" by (auto split: predicate_decl.splits)
+      
+      from y
+      obtain py ny vy  where
+        py: "case_predicate_decl Pair py = y"
+        "py \<in> set (predicates D)"
+        "py = PredDecl ny vy"
+        "y = (ny, vy)" by (auto split: predicate_decl.splits)
+      
+      from xy px py
+      have "ny = nx" by simp
+
+      have "vx = vy" using wf_domain[simplified wf_domain_def] 
+      with wf_domain px py
+      show "x = y" using distinct_preds  sorry
+ 
+    qed
+  qed
+  ultimately
+  show "sig n = Some ts" unfolding sig_def by (auto intro: map_of_is_SomeI)
+qed
+  subgoal
+  apply (subst (asm) sig_def)
+   apply (drule map_of_SomeD)
+    by (auto split: predicate_decl.splits) 
+  subgoal
+  apply (subst sig_def)
+  apply (rule map_of_is_SomeI)
+  using wf_domain[simplified wf_domain_def, THEN conjunct2, THEN conjunct1]
+  find_theorems intro
+  
+    
+lemma wf_inst_with_objs_of_type:
+  fixes n params d cond eff
+  defines "a \<equiv> Durative_Action_Schema n params d cond eff"  
+  assumes "a \<in> set (actions D)"
+      and "(map snd params, args) \<in> ltos"
+shows "wf_ground_action (inst_snap_action a args ta)"
+proof -
+  have "action_params_match a args" using typed_args_correct assms(3)
+    unfolding action_params_match_def parameters_def using assms(1) by simp
+  moreover
+  have "wf_action_schema a" using wf_domain unfolding wf_domain_def using assms(2) by blast
+  ultimately
+  show ?thesis using wf_inst_durative_action_schema assms(1) by blast
+qed
+
+lemma "wf_pred_atom objT (n, vs) \<longleftrightarrow> predAtm n vs \<in> preds"
+  apply (rule iffI)
+  subgoal
+    apply (subst (asm) wf_pred_atom.simps)
+    apply (subst preds_def)
+    apply (auto split: option.splits)
+    subgoal for ts
+      unfolding sig_def 
+
+lemma "wf_fmla_atom objT f \<longleftrightarrow> f \<in> props"
+  sorry
+
+
+lemma 
+  assumes "wf_effect objT eff"
+  shows "effect_preds eff \<subseteq> preds"
+  using assms unfolding preds_def
+
+lemma 
+  assumes "wf_ground_action a"
+  shows "ga_preds a \<subseteq> preds" 
+  sorry
+lemma 
+  assumes "(n, s, i, e, c) \<in> pddl_durative_actions" 
+  shows"ga_preds s \<subseteq> preds \<and> ga_preds i \<subseteq> preds \<and> ga_preds e \<subseteq> preds"
+proof (intro conjI)
+  
+qed
+
+end
+
+context wf_ast_problem
+begin
+
+sublocale temp_planning_problem props acts initial_state goal_imp at_start_imp at_end_imp over_all_imp lower_impl upper_impl snap_action_pre snap_action_adds snap_action_dels 0
+proof 
+  show "initial_state \<subseteq> props"
+  proof -
+    
+    from wf_problem
+    have "\<forall>f \<in> set (init P). wf_fmla_atom objT f \<or> wf_func_assign f" unfolding wf_problem_def by simp
+    moreover
+    have "\<forall>p. is_predAtom p \<longrightarrow> \<not>(wf_func_assign p)"
+      apply (rule allI) 
+      subgoal for p apply (cases p) 
+        subgoal for x apply (cases x) by auto 
+        by auto
+      done
+    ultimately
+    have "\<forall>p \<in> I. wf_fmla_atom objT p" unfolding I_def by auto
+    moreover
+    have 1: "sig a = Some ts \<Longrightarrow> PredDecl a ts \<in> set (predicates D)" for a ts
+      apply (subst (asm) sig_def)
+      apply (drule map_of_SomeD)
+      by (auto split: predicate_decl.splits) 
+  
+    have "is_of_type objT obj ty \<Longrightarrow> obj \<in> objs" for obj ty
+      unfolding objs_def objT_def constT_def is_of_type_def 
+      apply (erule case_optionE)
+       apply simp
+      subgoal for vT
+        apply (subst (asm) map_of_append[symmetric])
+        apply (drule map_of_SomeD)
+        by auto
+      done
+    hence 2: "is_of_type objT obj ty \<Longrightarrow> obj \<in> objs \<and> is_of_type objT obj ty " for obj ty
+      by simp
+    have 3: "\<forall>f. wf_fmla_atom objT f \<longrightarrow> f \<in> props"
+      apply (rule allI; rule impI)
+      subgoal for f
+        apply (induction f)
+        subgoal for x
+          apply (induction x)
+          subgoal for a vs
+            unfolding props_def propositions_def preds_def
+            apply (subst (asm) wf_fmla_atom.simps)
+            apply (subst (asm) wf_pred_atom.simps)
+            apply (erule case_optionE)
+             apply auto[1]
+            subgoal for ts
+              apply (rule UnI1, rule UnI1, rule UnI1, rule UnI2)
+              unfolding ltos_def tos_def 
+              apply (subst is_obj_of_type_alt) 
+              apply (rule imageI)
+              apply (drule 1)
+              apply (drule list_all2_mono[OF _ 2])
+               apply assumption
+              apply simp
+              apply (rule exI[where x = ts])
+              apply auto
+              apply (subst list_all2_iff)
+              apply (subst (asm) list_all2_iff)
+              apply (rule conjI)
+               apply simp
+              apply (rule ballI)
+              subgoal for x
+                apply (induction x)
+                subgoal for x y
+                  apply (drule conjunct2)
+                  apply (drule bspec[where x = "(y, x)"])
+                   apply (subst in_set_zip)
+                   apply (subst (asm) in_set_zip)
+                  by auto
+                done
+              done
+            done
+          by auto
+        by auto
+      done
+    ultimately
+    show ?thesis unfolding initial_state_def props_def initial_state'_def propositions_def by blast
+  qed
+  show "goal_imp \<subseteq> props" unfolding goal_imp_def props_def by simp
+  show "let snap_props = \<lambda>s. snap_action_pre s \<union> snap_action_adds s \<union> snap_action_dels s
+    in \<forall>a\<in>acts. snap_props (at_start_imp a) \<subseteq> props \<and> snap_props (at_end_imp a) \<subseteq> props \<and> over_all_imp a \<subseteq> props"
+  proof -
+    define snap_props where [simp]: "snap_props = (\<lambda>s. snap_action_pre s \<union> snap_action_adds s \<union> snap_action_dels s)"
+    have "snap_props (at_start_imp a) \<subseteq> props \<and> snap_props (at_end_imp a) \<subseteq> props \<and> over_all_imp a \<subseteq> props" 
+      if a_in_acts: "a \<in> acts" for a
+    proof -
+      consider "a \<in> prop_actions" | "a \<in> goal_actions" using a_in_acts unfolding acts_def by blast
+      thus ?thesis
+      proof cases
+        case 1
+        then obtain n s s' inv inv' e e' c where
+          "a = (n, s, inv, e, c)" 
+          "s \<in> snap_actions s'"
+          "inv \<in> snap_actions inv'"
+          "e \<in> snap_actions e'"
+          "(n, s', inv', e', c) \<in> pddl_actions" 
+          unfolding prop_actions_def by blast
+        show ?thesis 
+        proof (intro conjI)
+          from 1
+          
+        qed
+      next
+        case 2
+        show ?thesis 
+        proof (intro conjI)
+
+        qed
+      qed
+    qed
+    thus ?thesis by auto
+  qed
+qed
 end
 
 end
